Rename EpsilonElimination

PumpingCfg/EpsilonElimination.lean
@@ -8,6 +8,19 @@ import Mathlib.Computability.ContextFreeGrammar
 import PumpingCfg.Utils
 import PumpingCfg.CountingSteps
 
+namespace ContextFreeRule
+universe uT uN
+
+variable {T : Type uT} {N : Type uN}
+
+lemma Rewrites.empty {u : List (Symbol T N)} {r : ContextFreeRule T N}
+    (hu : r.Rewrites u []) :
+    r.output = [] := by
+  obtain ⟨_, _, -, _⟩ := hu.exists_parts
+  simp_all
+
+end ContextFreeRule
+
 namespace ContextFreeGrammar
 
 universe uT uN
@@ -110,11 +123,11 @@ lemma DerivesIn.empty_of_append_right {m : ℕ} {u v : List (Symbol T g.NT)}
   apply empty_of_append_right_aux <;> tauto
 
 lemma DerivesIn.empty_of_append {u v w : List (Symbol T g.NT)} {m : ℕ}
-    (huvwe : g.DerivesIn (u ++ v ++ w) [] m) :
+    (huvw : g.DerivesIn (u ++ v ++ w) [] m) :
     ∃ k ≤ m, g.DerivesIn v [] k := by
-  obtain ⟨m₁, hm₁n, huve⟩ := huvwe.empty_of_append_left
-  obtain ⟨m₂, hm₂n, hve⟩ := huve.empty_of_append_right
-  exact ⟨m₂, Nat.le_trans hm₂n hm₁n, hve⟩
+  obtain ⟨m₁, hm₁n, huv⟩ := huvw.empty_of_append_left
+  obtain ⟨m₂, hm₂n, hv⟩ := huv.empty_of_append_right
+  exact ⟨m₂, Nat.le_trans hm₂n hm₁n, hv⟩
 
 lemma NullableWord.empty_of_append {u v w : List (Symbol T g.NT)}
     (huvw : NullableWord (u ++ v ++ w)) :
@@ -150,22 +163,16 @@ lemma DerivesIn.mem_nullable {u : List (Symbol T g.NT)} {s : Symbol T g.NT} {m :
       obtain ⟨m', hmm, hse⟩ := ih hte hs
       exact ⟨m', hmm.trans hmn, hse⟩
 
-lemma rewrites_empty_output {u : List (Symbol T g.NT)} {r : ContextFreeRule T g.NT}
-    (hu : r.Rewrites u []) :
-    r.output = [] := by
-  obtain ⟨_, _, -, _⟩ := hu.exists_parts
-  simp_all
-
 lemma Derives.append_left_trans {u v w x: List (Symbol T g.NT)} (huv : g.Derives u v)
     (hwx : g.Derives w x) :
     g.Derives (w ++ u) (x ++ v) :=
   (huv.append_left _).trans (hwx.append_right _)
 
-lemma rewrites_produces {r : ContextFreeRule T g.NT} (hrg : r ∈ g.rules) :
+lemma Produces.input_output {r : ContextFreeRule T g.NT} (hrg : r ∈ g.rules) :
     g.Produces [.nonterminal r.input] r.output :=
   ⟨r, hrg, ContextFreeRule.Rewrites.input_output⟩
 
-lemma nullable_not_terminal {t : T} {u : List (Symbol T g.NT)} :
+lemma NullableWord.cons_terminal {t : T} {u : List (Symbol T g.NT)} :
     ¬ NullableWord (Symbol.terminal t :: u) := by
   by_contra htu
   change g.Derives ([Symbol.terminal t] ++ u) [] at htu
@@ -177,7 +184,7 @@ lemma nullable_not_terminal {t : T} {u : List (Symbol T g.NT)} :
     | cons _ hts =>
       cases hts
 
-lemma Derives.empty_empty {u : List (Symbol T g.NT)} (hu : g.Derives [] u) : u = [] := by
+lemma Derives.of_empty {u : List (Symbol T g.NT)} (hu : g.Derives [] u) : u = [] := by
   induction hu with
   | refl => rfl
   | tail _ hp _ =>
@@ -222,7 +229,7 @@ lemma NullableWord.nullableNonTerminal {u : List (Symbol T g.NT)} {s : Symbol T 
     cases hsu with
     | head =>
       cases a with
-      | terminal => exact (nullable_not_terminal hu).elim
+      | terminal => exact hu.cons_terminal.elim
       | nonterminal n => exact ⟨n, rfl, hu.empty_of_append_left⟩
     | tail _ hsu =>
       apply ih _ hsu
@@ -275,7 +282,7 @@ lemma NullableRelated.derives {u v : List (Symbol T g.NT)} (huv : NullableRelate
     rw [← List.singleton_append]
     exact Derives.append_left_trans ih hnt
 
-lemma NullableRelated.empty_nullable {u : List (Symbol T g.NT)} (hu : NullableRelated [] u) :
+lemma NullableRelated.empty_nullableWord {u : List (Symbol T g.NT)} (hu : NullableRelated [] u) :
     NullableWord u := by
   induction u with
   | nil => rfl
@@ -283,22 +290,10 @@ lemma NullableRelated.empty_nullable {u : List (Symbol T g.NT)} (hu : NullableRe
     | empty_left _ hsl => exact hsl
     | cons_nterm_nullable hl hn => exact (Derives.append_right hn l).trans (ih hl)
 
-lemma NullableRelated.empty_empty {u : List (Symbol T g.NT)} (hu : NullableRelated u []) :
+lemma NullableRelated.empty_right {u : List (Symbol T g.NT)} (hu : NullableRelated u []) :
     u = [] := by
   cases hu
   rfl
-
-lemma NullableRelated.append_nullable' {u v w : List (Symbol T g.NT)}
-    (hvu : NullableRelated v u) (hw : NullableWord w) :
-    NullableRelated v (w ++ u) := by
-  induction w generalizing u v with
-  | nil => rwa [List.nil_append]
-  | cons a l ih =>
-    rw [←List.singleton_append] at hw
-    obtain ⟨_, rfl, hnt⟩ := hw.nullableNonTerminal (List.mem_cons_self a l)
-    constructor
-    · exact ih hvu (NullableWord.empty_of_append_right hw)
-    · exact hnt
 
 lemma NullableRelated.append_nullable_left {u v w: List (Symbol T g.NT)}
     (huv : NullableRelated u v) (hw : NullableWord w) :
@@ -310,13 +305,13 @@ lemma NullableRelated.append_nullable_left {u v w: List (Symbol T g.NT)}
     obtain ⟨_, rfl, hnt⟩ := hw.nullableNonTerminal (List.mem_cons_self a l)
     exact NullableRelated.cons_nterm_nullable (ih huv (NullableWord.empty_of_append_right hw)) hnt
 
-lemma NullableRelated.append {u₁ u₂ v₁ v₂ : List (Symbol T g.NT)}
+lemma nullable_related_append {u₁ u₂ v₁ v₂ : List (Symbol T g.NT)}
     (hv : NullableRelated v₁ v₂) (hu : NullableRelated u₁ u₂) :
     NullableRelated (v₁ ++ u₁) (v₂ ++ u₂) := by
   induction hv with
   | empty_left v₂ hv => exact hu.append_nullable_left hv
-  | cons_term _ t ih => exact cons_term ih t
-  | cons_nterm_match _ n ih => exact cons_nterm_match ih n
+  | cons_term _ t ih => exact NullableRelated.cons_term ih t
+  | cons_nterm_match _ n ih => exact NullableRelated.cons_nterm_match ih n
   | cons_nterm_nullable _ hnt ih => exact NullableRelated.cons_nterm_nullable ih hnt
 
 lemma NullableRelated.append_split {u v w : List (Symbol T g.NT)}
@@ -333,7 +328,7 @@ lemma NullableRelated.append_split {u v w : List (Symbol T g.NT)}
       have hvw : NullableRelated [] (l ++ w) := by
         constructor
         rw [← List.singleton_append, List.append_assoc] at huvw
-        exact NullableWord.empty_of_append_right huvw.empty_nullable
+        exact NullableWord.empty_of_append_right huvw.empty_nullableWord
       obtain ⟨_, _, heq, _, hw⟩ := ih hvw
       simp at heq
       constructor
@@ -345,7 +340,7 @@ lemma NullableRelated.append_split {u v w : List (Symbol T g.NT)}
           apply Derives.trans
           · apply Derives.append_right
             assumption
-          · exact hvw.empty_nullable.empty_of_append_left
+          · exact hvw.empty_nullableWord.empty_of_append_left
       · exact heq.right ▸ hw
     | cons sᵤ u =>
       cases huvw with
@@ -380,22 +375,22 @@ variable {N : Type uN} [DecidableEq N]
 
 /-- Check if a symbol is nullable (w.r.t. to set of nullable symbols `p`), i.e.,
  `symbol_is_nullable p s` only holds if `s` is a nonterminal and it is in `p` -/
-def symbol_is_nullable (p : Finset N) (s : Symbol T N) : Bool :=
+def symbolIsNullable (p : Finset N) (s : Symbol T N) : Bool :=
   match s with
   | Symbol.terminal _ => False
   | Symbol.nonterminal n => n ∈ p
 
 /-- A rule is nullable if all output symbols are nullable -/
-def rule_is_nullable (p : Finset N) (r : ContextFreeRule T N) : Bool :=
-  ∀ s ∈ r.output, symbol_is_nullable p s
+def ruleIsNullable (p : Finset N) (r : ContextFreeRule T N) : Bool :=
+  ∀ s ∈ r.output, symbolIsNullable p s
 
 /-- Add the input of a rule as a nullable symbol to `p` if the rule is nullable -/
-def add_if_nullable (r : ContextFreeRule T N) (p : Finset N) : Finset N :=
-  if rule_is_nullable p r then insert r.input p else p
+def addIfNullable (r : ContextFreeRule T N) (p : Finset N) : Finset N :=
+  if ruleIsNullable p r then insert r.input p else p
 
-lemma add_if_nullable_subset (r : ContextFreeRule T N) (p : Finset N) :
-  p ⊆ (add_if_nullable r p) := by
-  unfold add_if_nullable
+lemma sub_addIfNullable (r : ContextFreeRule T N) (p : Finset N) :
+  p ⊆ (addIfNullable r p) := by
+  unfold addIfNullable
   split <;> simp
 
 variable {g : ContextFreeGrammar.{uN, uT} T} [DecidableEq g.NT]
@@ -404,7 +399,7 @@ variable {g : ContextFreeGrammar.{uN, uT} T} [DecidableEq g.NT]
 noncomputable def generators (g : ContextFreeGrammar.{uN, uT} T) [DecidableEq g.NT] : Finset g.NT :=
   (g.rules.toList.map (fun r ↦ r.input)).toFinset
 
-lemma input_in_generators {r : ContextFreeRule T g.NT} (hrg : r ∈ g.rules) :
+lemma input_mem_generators {r : ContextFreeRule T g.NT} (hrg : r ∈ g.rules) :
   r.input ∈ g.generators := by
   unfold generators
   rw [← Finset.mem_toList] at hrg
@@ -420,85 +415,68 @@ lemma input_in_generators {r : ContextFreeRule T g.NT} (hrg : r ∈ g.rules) :
     · right
       exact ih c2
 
-lemma nonterminal_in_generators {v : g.NT} {r : ContextFreeRule T g.NT} (hrg : r ∈ g.rules)
-    (hv : r.input = v) :
-    v ∈ g.generators := by
-  unfold generators
-  rw [← Finset.mem_toList] at hrg
-  revert hrg
-  induction g.rules.toList with
-  | nil => simp
-  | cons _ _ ih =>
-    simp only [List.mem_toFinset, List.mem_map, List.mem_cons, List.map_cons, List.toFinset_cons,
-      Finset.mem_insert] at ih ⊢
-    rintro (c1 | c2)
-    · left
-      rw [← hv, c1]
-    · right
-      exact ih c2
-
-lemma add_if_nullable_subset_generators {r : ContextFreeRule T g.NT} {p : Finset g.NT}
+lemma addIfNullable_sub_generators {r : ContextFreeRule T g.NT} {p : Finset g.NT}
     (hpg : p ⊆ g.generators) (hrg : r ∈ g.rules) :
-    add_if_nullable r p ⊆ g.generators := by
-  unfold add_if_nullable
+    addIfNullable r p ⊆ g.generators := by
+  unfold addIfNullable
   split
-  · exact Finset.insert_subset (input_in_generators hrg) hpg
+  · exact Finset.insert_subset (input_mem_generators hrg) hpg
   · exact hpg
 
 /-- Single round of fixpoint iteration; adds `r.input` to the set of nullable symbols if all symbols in
  `r.output` are nullable -/
-noncomputable def add_nullables (p : Finset g.NT) : Finset g.NT :=
-  g.rules.toList.attach.foldr (fun ⟨r, _⟩ ↦ add_if_nullable r) p
+noncomputable def addNullables (p : Finset g.NT) : Finset g.NT :=
+  g.rules.toList.attach.foldr (fun ⟨r, _⟩ ↦ addIfNullable r) p
 
-lemma add_nullables_sub_generators (p : Finset g.NT) (hpg : p ⊆ g.generators) :
-    add_nullables p ⊆ g.generators := by
-  unfold add_nullables
+lemma addNullables_sub_generators (p : Finset g.NT) (hpg : p ⊆ g.generators) :
+    addNullables p ⊆ g.generators := by
+  unfold addNullables
   induction g.rules.toList.attach with
   | nil => simpa using hpg
-  | cons a _ ih => exact add_if_nullable_subset_generators ih (Finset.mem_toList.1 a.2)
+  | cons a _ ih => exact addIfNullable_sub_generators ih (Finset.mem_toList.1 a.2)
 
-lemma nullable_sub_add_nullables (p : Finset g.NT) : p ⊆ (add_nullables p) := by
-  unfold add_nullables
+lemma sub_addNullables (p : Finset g.NT) : p ⊆ (addNullables p) := by
+  unfold addNullables
   induction g.rules.toList.attach with
   | nil => simp
   | cons a _ ih =>
     apply subset_trans ih
-    apply add_if_nullable_subset a.1
+    apply sub_addIfNullable a.1
 
 lemma generators_limits_nullable (p : Finset g.NT) (hpg : p ⊆ g.generators)
-    (hne : p ≠ add_nullables p) :
-    (g.generators).card - (add_nullables p).card < (g.generators).card - p.card := by
-  have h := HasSubset.Subset.ssubset_of_ne (nullable_sub_add_nullables p) hne
+    (hne : p ≠ addNullables p) :
+    (g.generators).card - (addNullables p).card < (g.generators).card - p.card := by
+  have h := HasSubset.Subset.ssubset_of_ne (sub_addNullables p) hne
   apply Nat.sub_lt_sub_left
   · apply Nat.lt_of_lt_of_le
     · apply Finset.card_lt_card h
-    · exact Finset.card_le_card (add_nullables_sub_generators p hpg)
+    · exact Finset.card_le_card (addNullables_sub_generators p hpg)
   · apply Finset.card_lt_card h
 
 /-- Fixpoint iteration computing the set of nullable symbols of `g`. -/
-noncomputable def add_nullables_iter (p : Finset g.NT) (hpg : p ⊆ g.generators) :=
-  let nullable' := add_nullables p
+noncomputable def addNullablesIter (p : Finset g.NT) (hpg : p ⊆ g.generators) :=
+  let nullable' := addNullables p
   if p = nullable' then
     p
   else
-    add_nullables_iter nullable' (add_nullables_sub_generators p hpg)
+    addNullablesIter nullable' (addNullables_sub_generators p hpg)
   termination_by ((g.generators).card - p.card)
   decreasing_by
     rename_i h
     exact generators_limits_nullable p hpg h
 
 /-- Compute the least-fixpoint of `add_nullable_iter`, i.e., all (and only) nullable symbols -/
-noncomputable def compute_nullables (g : ContextFreeGrammar.{uN, uT} T) [DecidableEq g.NT] :=
-  add_nullables_iter ∅ g.generators.empty_subset
+noncomputable def computeNullables (g : ContextFreeGrammar.{uN, uT} T) [DecidableEq g.NT] :=
+  addNullablesIter ∅ g.generators.empty_subset
 
 -- ********************************************************************** --
--- Only If direction of the main correctness theorem of compute_nullables --
+-- Only If direction of the main correctness theorem of computeNullables --
 -- ********************************************************************** --
 
-lemma rule_is_nullable_correct (p : Finset g.NT) (r : ContextFreeRule T g.NT) (hrg : r ∈ g.rules)
-    (hn : ∀ v ∈ p, NullableNonTerminal v) (hr : rule_is_nullable p r) :
+lemma ruleIsNullable_NullableNonTerminal (p : Finset g.NT) (r : ContextFreeRule T g.NT)
+    (hrg : r ∈ g.rules) (hn : ∀ v ∈ p, NullableNonTerminal v) (hr : ruleIsNullable p r) :
     NullableNonTerminal r.input := by
-  unfold rule_is_nullable at hr
+  unfold ruleIsNullable at hr
   unfold NullableNonTerminal
   have h1 : g.Produces [Symbol.nonterminal r.input] r.output := by
     use r, hrg
@@ -510,50 +488,49 @@ lemma rule_is_nullable_correct (p : Finset g.NT) (r : ContextFreeRule T g.NT) (h
   intro v hvin
   rw [decide_eq_true_eq] at hr
   specialize hr v hvin
-  cases v <;> simp [symbol_is_nullable] at hr
+  cases v <;> simp [symbolIsNullable] at hr
   exact hn _ hr
 
-lemma add_nullables_nullable (p : Finset g.NT) (hp : ∀ v ∈ p, NullableNonTerminal v) :
-    ∀ v ∈ add_nullables p, NullableNonTerminal v := by
-  unfold add_nullables
+lemma addNullables_mem_nullableNonTerminal (p : Finset g.NT) (hp : ∀ v ∈ p, NullableNonTerminal v) :
+    ∀ v ∈ addNullables p, NullableNonTerminal v := by
+  unfold addNullables
   induction g.rules.toList.attach with
   | nil => exact hp
   | cons a l ih =>
-    simp only [List.foldr_cons, Finset.mem_toList, List.foldr_subtype, add_if_nullable]
+    simp only [List.foldr_cons, Finset.mem_toList, List.foldr_subtype, addIfNullable]
     split <;> rename_i hd
     · simp only [Finset.mem_insert, forall_eq_or_imp]
       constructor
-      · apply rule_is_nullable_correct _ _ (Finset.mem_toList.1 a.2) ih
+      · apply ruleIsNullable_NullableNonTerminal _ _ (Finset.mem_toList.1 a.2) ih
         simpa using hd
       · simpa using ih
     · simpa using ih
 
-lemma add_nullables_iter_only_nullable (p : Finset g.NT) (hpg : p ⊆ g.generators)
+lemma addNullablesIter_only_nullableNonTerminal (p : Finset g.NT) (hpg : p ⊆ g.generators)
     (hp : ∀ v ∈ p, NullableNonTerminal v) :
-    ∀ v ∈ (add_nullables_iter p hpg), NullableNonTerminal v:= by
-  unfold add_nullables_iter
+    ∀ v ∈ (addNullablesIter p hpg), NullableNonTerminal v:= by
+  unfold addNullablesIter
   intro
   simp only
   split
   · tauto
-  · apply add_nullables_iter_only_nullable (add_nullables p)
-          (add_nullables_sub_generators p hpg)
-          (add_nullables_nullable p hp)
+  · apply addNullablesIter_only_nullableNonTerminal (addNullables p)
+          (addNullables_sub_generators p hpg)
+          (addNullables_mem_nullableNonTerminal p hp)
   termination_by ((g.generators).card - p.card)
   decreasing_by
     rename_i h
     exact generators_limits_nullable p hpg h
 
 -- ***************************************************************** --
--- If direction of the main correctness theorem of compute_nullables --
+-- If direction of the main correctness theorem of computeNullables --
 -- ***************************************************************** --
 
-lemma subset_add_if_nullable_subset {r: ContextFreeRule T g.NT} {p₁ p₂ : Finset g.NT}
-    (hpp : p₁ ⊆ p₂) :
-    add_if_nullable r p₁ ⊆ add_if_nullable r p₂ := by
+lemma addIfNullable_monotone {r: ContextFreeRule T g.NT} {p₁ p₂ : Finset g.NT} (hpp : p₁ ⊆ p₂) :
+    addIfNullable r p₁ ⊆ addIfNullable r p₂ := by
   intro v hvin
-  unfold add_if_nullable rule_is_nullable at hvin ⊢
-  by_cases hsr : decide (∀ s ∈ r.output, symbol_is_nullable p₁ s) = true <;>
+  unfold addIfNullable ruleIsNullable at hvin ⊢
+  by_cases hsr : decide (∀ s ∈ r.output, symbolIsNullable p₁ s) = true <;>
     simp [hsr] at hvin; simp at hsr
   · split <;> rename_i hsr'; simp at hsr'
     · cases hvin with
@@ -564,7 +541,7 @@ lemma subset_add_if_nullable_subset {r: ContextFreeRule T g.NT} {p₁ p₂ : Fin
         exact Finset.mem_insert_of_mem (hpp hv)
     · cases hvin with
       | inl h'' =>
-        unfold symbol_is_nullable at hsr' hsr
+        unfold symbolIsNullable at hsr' hsr
         simp at hsr' hsr -- TODO
         obtain ⟨s, hsin, hs⟩ := hsr'
         specialize hsr s
@@ -580,19 +557,19 @@ lemma subset_add_if_nullable_subset {r: ContextFreeRule T g.NT} {p₁ p₂ : Fin
     · exact Finset.mem_insert_of_mem (hpp hvin)
     · exact hpp hvin
 
-private lemma add_if_nullable_subset_rec {l : List (ContextFreeRule T g.NT)} {p : Finset g.NT} :
-    p ⊆ List.foldr add_if_nullable p l := by
+private lemma sub_addIfNullable_rec {l : List (ContextFreeRule T g.NT)} {p : Finset g.NT} :
+    p ⊆ List.foldr addIfNullable p l := by
   induction l with
   | nil => rfl
   | cons _ _ ih =>
     simp
     apply Finset.Subset.trans ih
-    apply add_if_nullable_subset
+    apply sub_addIfNullable
 
-lemma nullable_in_add_nullables {r : ContextFreeRule T g.NT} {p : Finset g.NT}
-    (hr : rule_is_nullable p r) (hrg : r ∈ g.rules) :
-    r.input ∈ add_nullables p := by
-  unfold add_nullables
+lemma nullable_input_mem_addNullables {r : ContextFreeRule T g.NT} {p : Finset g.NT}
+    (hr : ruleIsNullable p r) (hrg : r ∈ g.rules) :
+    r.input ∈ addNullables p := by
+  unfold addNullables
   have hrg := List.mem_attach g.rules.toList ⟨r, (Finset.mem_toList.2 hrg)⟩
   revert r p
   induction g.rules.toList.attach with
@@ -602,64 +579,64 @@ lemma nullable_in_add_nullables {r : ContextFreeRule T g.NT} {p : Finset g.NT}
   | cons _ _ ih =>
     intro r' nullable h hr' hr''
     cases hr'' <;> simp at ih ⊢
-    · apply Finset.mem_of_subset (subset_add_if_nullable_subset add_if_nullable_subset_rec)
-      simp [add_if_nullable, h]
+    · apply Finset.mem_of_subset (addIfNullable_monotone sub_addIfNullable_rec)
+      simp [addIfNullable, h]
     · rename_i hr''
-      exact Finset.mem_of_subset (add_if_nullable_subset _ _) (ih h hr' hr'')
+      exact Finset.mem_of_subset (sub_addIfNullable _ _) (ih h hr' hr'')
 
-lemma add_nullable_add_nullable_iter (p: Finset g.NT) (hpg : p ⊆ g.generators) :
-    add_nullables_iter p hpg = add_nullables (add_nullables_iter p hpg) := by
-  unfold add_nullables_iter
+lemma addNullablesIter_fixpoint (p: Finset g.NT) (hpg : p ⊆ g.generators) :
+    addNullablesIter p hpg = addNullables (addNullablesIter p hpg) := by
+  unfold addNullablesIter
   dsimp only
   split
   · assumption
-  · apply add_nullable_add_nullable_iter
+  · apply addNullablesIter_fixpoint
   termination_by ((g.generators).card - p.card)
   decreasing_by
     rename_i h
     exact generators_limits_nullable p hpg h
 
-lemma nullable_in_compute_nullables (p : Finset g.NT) (hpg : p ⊆ g.generators)
+lemma nullable_mem_addNullablesIter (p : Finset g.NT) (hpg : p ⊆ g.generators)
     (n : g.NT) (m : ℕ) (hvgm : g.DerivesIn [Symbol.nonterminal n] [] m) :
-    n ∈ add_nullables_iter p hpg := by
+    n ∈ addNullablesIter p hpg := by
   cases m with
   | zero => cases hvgm
   | succ m =>
     obtain ⟨u, hwu, hue⟩ := hvgm.head_of_succ
     obtain ⟨r, hrg, hwu⟩ := hwu
-    have hr : rule_is_nullable (add_nullables_iter p hpg) r := by
+    have hr : ruleIsNullable (addNullablesIter p hpg) r := by
       have hur : u = r.output := by
         obtain ⟨p, q, hv, hu⟩ := hwu.exists_parts
         cases p <;> simp at hv
         cases q <;> simp at hv
         simpa using hu
-      unfold rule_is_nullable
+      unfold ruleIsNullable
       rw [decide_eq_true_eq]
       intro s hs
       rw [←hur] at hs
       obtain ⟨v', hv'⟩ := hue.nullable_mem_nonterminal hs
-      unfold symbol_is_nullable
+      unfold symbolIsNullable
       rw [hv', decide_eq_true_eq]
       have ⟨_, _, _⟩ := hue.mem_nullable hs
-      apply nullable_in_compute_nullables
+      apply nullable_mem_addNullablesIter
       rwa [←hv']
     have hv : n = r.input := by
       obtain ⟨p, q, hu, _⟩ := hwu.exists_parts
       cases p <;> simp at hu
       cases q <;> simp at hu
       exact hu
-    rw [add_nullable_add_nullable_iter, hv]
-    exact nullable_in_add_nullables hr hrg
+    rw [addNullablesIter_fixpoint, hv]
+    exact nullable_input_mem_addNullables hr hrg
 
 -- Main correctness theorem of computing all nullable symbols --
-lemma compute_nullables_iff (n : g.NT) : n ∈ compute_nullables g ↔ NullableNonTerminal n := by
+lemma computeNullables_iff (n : g.NT) : n ∈ computeNullables g ↔ NullableNonTerminal n := by
   constructor
   · intro hng
-    apply add_nullables_iter_only_nullable _ _ _ _ hng
+    apply addNullablesIter_only_nullableNonTerminal _ _ _ _ hng
     tauto
   · intro hn
     obtain ⟨m, hgnm⟩ := (derives_iff_derivesIn _ _ _).1 hn
-    apply nullable_in_compute_nullables
+    apply nullable_mem_addNullablesIter
     exact hgnm
 
 end ComputeNullables
@@ -673,94 +650,94 @@ section EliminateEmpty
 variable {N : Type uN} [DecidableEq N]
 
 /-- Compute all possible combinations of leaving out nullable nonterminals from `u` -/
-def remove_nullable (p : Finset N) (u : List (Symbol T N)) :=
+def nullableCombinations (p : Finset N) (u : List (Symbol T N)) : List (List (Symbol T N)) :=
   match u with
   | [] => [[]]
   | x :: s =>
     match x with
     | Symbol.nonterminal n =>
-      (if n ∈ p then remove_nullable p s else []) ++
-        (remove_nullable p s).map (x :: ·)
-    | Symbol.terminal _ => (remove_nullable p s).map (x :: ·)
+      (if n ∈ p then nullableCombinations p s else []) ++
+        (nullableCombinations p s).map (x :: ·)
+    | Symbol.terminal _ => (nullableCombinations p s).map (x :: ·)
 
 /-- Computes all variations of leaving out nullable symbols (except the empty string) of `r` -/
-def remove_nullable_rule (p : Finset N) (r: ContextFreeRule T N) :=
+def removeNullableRule (p : Finset N) (r: ContextFreeRule T N) :=
   let fltrmap : List (Symbol T N) → Option (ContextFreeRule T N)
     | [] => Option.none
     | h :: t => ContextFreeRule.mk r.input (h :: t)
-  (remove_nullable p r.output).filterMap fltrmap
+  (nullableCombinations p r.output).filterMap fltrmap
 
 variable {g : ContextFreeGrammar.{uN, uT} T} [DecidableEq g.NT]
 
 /-- Compute all variations of leaving out nullable symbols (except the empty string) of `g`s rules -/
-noncomputable def remove_nullables (p : Finset g.NT) [DecidableEq T] :=
-  (g.rules.toList.map (remove_nullable_rule p)).flatten.toFinset
+noncomputable def removeNullables (p : Finset g.NT) [DecidableEq T] :=
+  (g.rules.toList.map (removeNullableRule p)).flatten.toFinset
 
 /- Given `g`, computes a new grammar in which all rules deriving `[]` are removed and all
  rules in `g` have a set of corresponding rules in g' in which some nullable symbols do not appear
  in the output. For example if `r: V -> ABC` is in `g` and `A` and `B` are nullable, the rules
  `r₁: V -> ABC`, `r₂: V -> BC`, `r₃: V -> AC`, and `r₄: V -> C` will be in `g.eliminate_empty` -/
-noncomputable def eliminate_empty (g : ContextFreeGrammar.{uN, uT} T) [DecidableEq g.NT]
+noncomputable def eliminateEmpty (g : ContextFreeGrammar.{uN, uT} T) [DecidableEq g.NT]
     [DecidableEq T] :=
-  ContextFreeGrammar.mk g.NT g.initial (remove_nullables g.compute_nullables)
+  ContextFreeGrammar.mk g.NT g.initial (removeNullables g.computeNullables)
 
 -- ******************************************************************** --
 -- Only If direction of the main correctness theorem of eliminate_empty --
 -- ******************************************************************** --
 
-lemma in_remove_nullable_rule {r r': ContextFreeRule T g.NT} {p : Finset g.NT}
-    (hrr : r' ∈ remove_nullable_rule p r) :
+lemma output_mem_removeNullableRule {r r': ContextFreeRule T g.NT} {p : Finset g.NT}
+    (hrr : r' ∈ removeNullableRule p r) :
     r'.output ≠ [] := by
-  unfold remove_nullable_rule at hrr
+  unfold removeNullableRule at hrr
   rw [List.mem_filterMap] at hrr
   obtain ⟨a, -, ha⟩ := hrr
   cases a <;> simp at ha
   rw [←ha]
   tauto
 
-lemma in_remove_not_epsilon {r : ContextFreeRule T g.NT} {p : Finset g.NT} [DecidableEq T]
-    (hr : r ∈ remove_nullables p) :
+lemma output_mem_removeNullables {r : ContextFreeRule T g.NT} {p : Finset g.NT} [DecidableEq T]
+    (hr : r ∈ removeNullables p) :
     r.output ≠ [] := by
-  unfold remove_nullables at hr
+  unfold removeNullables at hr
   rw [List.mem_toFinset, List.mem_flatten] at hr
   obtain ⟨l, hl, hr⟩ := hr
   rw [List.mem_map] at hl
   obtain ⟨r', _, hr'⟩ := hl
   rw [←hr'] at hr
-  exact in_remove_nullable_rule hr
+  exact output_mem_removeNullableRule hr
 
-lemma produces_not_epsilon {u v : List (Symbol T g.NT)} [DecidableEq T]
-    (huv : (g.eliminate_empty).Produces u v) :
+lemma eliminateEmpty_produces_not_empty {u v : List (Symbol T g.NT)} [DecidableEq T]
+    (huv : (g.eliminateEmpty).Produces u v) :
     v ≠ [] := by
   unfold Produces at huv
-  change ∃ r ∈ (remove_nullables g.compute_nullables), r.Rewrites u v at huv
+  change ∃ r ∈ (removeNullables g.computeNullables), r.Rewrites u v at huv
   obtain ⟨r, hrg, hr⟩ := huv
   intro hw
   rw [hw] at hr
-  exact in_remove_not_epsilon hrg (rewrites_empty_output hr)
+  exact output_mem_removeNullables hrg hr.empty
 
-lemma derives_not_epsilon {u v : List (Symbol T g.NT)} [DecidableEq T]
-    (huv : (g.eliminate_empty).Derives u v) (hune : u ≠ []) :
+lemma eliminateEmpty_derives_not_empty {u v : List (Symbol T g.NT)} [DecidableEq T]
+    (huv : (g.eliminateEmpty).Derives u v) (hune : u ≠ []) :
     v ≠ [] := by
-  change List (Symbol T g.eliminate_empty.NT) at u v
+  change List (Symbol T g.eliminateEmpty.NT) at u v
   induction huv using Derives.head_induction_on with
   | refl => exact hune
-  | head hp _ ih => exact ih (produces_not_epsilon (g := g) hp)
+  | head hp _ ih => exact ih (eliminateEmpty_produces_not_empty (g := g) hp)
 
--- Main proof of the only if direction: If the eliminate_empty grammar derives a string,
+-- Main proof of the only if direction: If the eliminateEmpty grammar derives a string,
 -- it is derivable in the original grammar
 
-lemma remove_nullable_related {u v: List (Symbol T g.NT)} (p : Finset g.NT)
-    (hn : ∀ x ∈ p, NullableNonTerminal x) (huv : u ∈ (remove_nullable p v)) :
+lemma mem_nullableCombinations_nullableRelated {u v: List (Symbol T g.NT)} (p : Finset g.NT)
+    (hn : ∀ x ∈ p, NullableNonTerminal x) (huv : u ∈ (nullableCombinations p v)) :
     NullableRelated u v := by
   induction v generalizing u with
   | nil =>
-    simp only [remove_nullable, List.mem_singleton] at huv
+    simp only [nullableCombinations, List.mem_singleton] at huv
     rw [huv]
   | cons s v ih =>
     cases s with
     | nonterminal n =>
-      simp [remove_nullable] at huv -- TODO
+      simp [nullableCombinations] at huv -- TODO
       cases huv with
       | inl hnu =>
         by_cases hnn : n ∈ p <;> simp only [hnn, false_and, true_and] at hnu
@@ -769,94 +746,87 @@ lemma remove_nullable_related {u v: List (Symbol T g.NT)} (p : Finset g.NT)
         obtain ⟨u', hu', rfl⟩ := huv
         exact NullableRelated.cons_nterm_match (ih hu') n
     | terminal t =>
-      rw [remove_nullable, List.mem_map] at huv
+      rw [nullableCombinations, List.mem_map] at huv
       obtain ⟨u', hu', rfl⟩ := huv
       exact NullableRelated.cons_term (ih hu') t
 
-lemma remove_nullable_rule_related {r': ContextFreeRule T g.NT} [DecidableEq T]
-    {r : ContextFreeRule T g.NT} {hrg : r ∈ remove_nullable_rule g.compute_nullables r'} :
+lemma mem_removeNullableRule_nullableRelated {r': ContextFreeRule T g.NT} [DecidableEq T]
+    {r : ContextFreeRule T g.NT} {hrg : r ∈ removeNullableRule g.computeNullables r'} :
     r.input = r'.input ∧ NullableRelated r.output r'.output := by
-  rw [remove_nullable_rule, List.mem_filterMap] at hrg
+  rw [removeNullableRule, List.mem_filterMap] at hrg
   obtain ⟨o, ho, ho'⟩ := hrg
   cases o <;> simp at ho'
   rw [←ho']
   constructor; rfl
-  apply remove_nullable_related
+  apply mem_nullableCombinations_nullableRelated
   intro
-  apply (compute_nullables_iff _).1 -- TODO
+  apply (computeNullables_iff _).1 -- TODO
   exact ho
 
-lemma eliminate_empty_rules [DecidableEq T] (r : ContextFreeRule T g.NT)
-    {hrg : r ∈ g.eliminate_empty.rules} :
+lemma mem_eliminateEmpty [DecidableEq T] (r : ContextFreeRule T g.NT)
+    {hrg : r ∈ g.eliminateEmpty.rules} :
     ∃ r' ∈ g.rules, r.input = r'.input ∧ NullableRelated r.output r'.output := by
-  unfold eliminate_empty remove_nullables at hrg
+  unfold eliminateEmpty removeNullables at hrg
   simp at hrg -- TODO
   obtain ⟨r', hgr', hr'⟩ := hrg
   use r', hgr'
-  apply remove_nullable_rule_related
+  apply mem_removeNullableRule_nullableRelated
   exact hr'
 
-lemma eliminate_empty_step_derives [DecidableEq T] {u v : List (Symbol T g.NT)}
-    (huv : g.eliminate_empty.Produces u v) :
+lemma eliminateEmpty_produces_to_derives [DecidableEq T] {u v : List (Symbol T g.NT)}
+    (huv : g.eliminateEmpty.Produces u v) :
     g.Derives u v := by
   obtain ⟨r, hrg, hr⟩ := huv
   obtain ⟨p, q, rfl, rfl⟩ := hr.exists_parts
   apply Derives.append_right
   apply Derives.append_left
-  obtain ⟨r', hr', hrr', hnrr'⟩ := @eliminate_empty_rules _ g _ _ r hrg
+  obtain ⟨r', hr', hrr', hnrr'⟩ := g.mem_eliminateEmpty r (hrg := hrg)
   rw [hrr']
-  exact (rewrites_produces hr').trans_derives hnrr'.derives
+  exact (Produces.input_output hr').trans_derives hnrr'.derives
 
-lemma eliminate_empty_implies [DecidableEq T] {u v : List (Symbol T g.NT)}
-    (huv : g.eliminate_empty.Derives u v) : g.Derives u v := by
-  change (List (Symbol T g.eliminate_empty.NT)) at u v
+lemma eliminateEmpty_derives_to_derives [DecidableEq T] {u v : List (Symbol T g.NT)}
+    (huv : g.eliminateEmpty.Derives u v) : g.Derives u v := by
+  change (List (Symbol T g.eliminateEmpty.NT)) at u v
   induction huv using Derives.head_induction_on with
   | refl => rfl
-  | head hp _ ih => exact Derives.trans (eliminate_empty_step_derives hp) ih
+  | head hp _ ih => exact Derives.trans (eliminateEmpty_produces_to_derives hp) ih
 
 -- *************************************************************** --
--- If direction of the main correctness theorem of eliminate_empty --
+-- If direction of the main correctness theorem of eliminateEmpty --
 -- *************************************************************** --
 
-lemma in_remove_nullable (p : Finset g.NT) (u : List (Symbol T g.NT)) : u ∈ remove_nullable p u := by
+lemma mem_nullableCombinations (p : Finset g.NT) (u : List (Symbol T g.NT)) : u ∈ nullableCombinations p u := by
   induction u with
   | nil =>
-    simp [remove_nullable]
+    simp [nullableCombinations]
   | cons s _ ih =>
     cases s with
-    | terminal t => simpa [remove_nullable] using ih
-    | nonterminal n => by_cases hn : n ∈ p <;> simp [remove_nullable, hn, ih]
+    | terminal t => simpa [nullableCombinations] using ih
+    | nonterminal n => by_cases hn : n ∈ p <;> simp [nullableCombinations, hn, ih]
 
-lemma nullableRelated_in_remove_nullable {p : Finset g.NT} {u v : List (Symbol T g.NT)}
+lemma nullableRelated_mem_removeNullable {p : Finset g.NT} {u v : List (Symbol T g.NT)}
     (hvu : NullableRelated v u) (hn : ∀ s, s ∈ p ↔ NullableNonTerminal s) :
-    v ∈ remove_nullable p u := by
+    v ∈ nullableCombinations p u := by
   induction u generalizing v with
   | nil =>
-    rw [hvu.empty_empty]
+    rw [hvu.empty_right]
     exact List.mem_singleton.2 rfl
   | cons a l ih =>
     cases a with
     | terminal t =>
-      simp [remove_nullable]
+      simp [nullableCombinations]
       cases hvu with
-      | @empty_left _ hvu =>
-        exfalso
-        exact nullable_not_terminal hvu
-      | cons_term hu =>
-        constructor
-        exact ⟨ih hu, rfl⟩
+      | @empty_left _ hvu => exact hvu.cons_terminal.elim
+      | cons_term hu => exact ⟨_, ih hu, rfl⟩
     | nonterminal n =>
-      simp only [remove_nullable, List.mem_append, List.mem_ite_nil_right, List.mem_map]
+      simp only [nullableCombinations, List.mem_append, List.mem_ite_nil_right, List.mem_map]
       cases hvu with
       | empty_left _ hu =>
         left
         rw [←List.singleton_append] at hu
         rw [hn]
         exact ⟨hu.empty_of_append_left, ih (NullableRelated.empty_left l hu.empty_of_append_right)⟩
-      | cons_nterm_match hu'u =>
-        right
-        constructor
-        exact ⟨ih hu'u, rfl⟩
+      | cons_nterm_match hu'u => exact Or.inr ⟨_, ih hu'u, rfl⟩
       | cons_nterm_nullable hvu hnn =>
         left
         rw [hn]
@@ -864,33 +834,31 @@ lemma nullableRelated_in_remove_nullable {p : Finset g.NT} {u v : List (Symbol T
 
 variable [DecidableEq T]
 
-lemma in_remove_nullables (p : Finset g.NT) (r : ContextFreeRule T g.NT) (hrg : r ∈ g.rules)
+lemma not_empty_mem_removeNullables (p : Finset g.NT) (r : ContextFreeRule T g.NT) (hrg : r ∈ g.rules)
     (hne : r.output ≠ []) :
-    r ∈ remove_nullables p := by
-  unfold remove_nullables
+    r ∈ removeNullables p := by
+  unfold removeNullables
   rw [List.mem_toFinset, List.mem_flatten]
-  use (remove_nullable_rule p r)
+  use (removeNullableRule p r)
   constructor
   · simp
     use r
-  · unfold remove_nullable_rule
+  · unfold removeNullableRule
     rw [List.mem_filterMap]
     use r.output
     constructor
-    · apply in_remove_nullable
+    · exact mem_nullableCombinations p r.output
     · obtain ⟨_, rₒ⟩ := r
-      cases rₒ
-      · contradiction
-      · rfl
+      cases rₒ <;> tauto
 
-lemma nullableRelated_rule_in_rules {r : ContextFreeRule T g.NT}
-    {u : List (Symbol T g.NT)} (hrg : r ∈ g.rules) (h : NullableRelated u r.output) (hneq : u ≠ []) :
-    { input := r.input, output := u } ∈ g.eliminate_empty.rules := by
-  unfold eliminate_empty
-  unfold remove_nullables
+lemma nullableRelated_mem_eliminateEmpty_rules {r : ContextFreeRule T g.NT} {u : List (Symbol T g.NT)}
+    (h : NullableRelated u r.output) (hrg : r ∈ g.rules) (hneq : u ≠ []) :
+    { input := r.input, output := u } ∈ g.eliminateEmpty.rules := by
+  unfold eliminateEmpty
+  unfold removeNullables
   rw [List.mem_toFinset, List.mem_flatten]
-  use (remove_nullable_rule g.compute_nullables r)
-  unfold remove_nullable_rule
+  use (removeNullableRule g.computeNullables r)
+  unfold removeNullableRule
   constructor
   · rw [List.mem_map]
     use r
@@ -900,14 +868,14 @@ lemma nullableRelated_rule_in_rules {r : ContextFreeRule T g.NT}
   · rw [List.mem_filterMap]
     use u
     constructor
-    · exact nullableRelated_in_remove_nullable h compute_nullables_iff
+    · exact nullableRelated_mem_removeNullable h computeNullables_iff
     · cases u
       · contradiction
       · rfl
 
-lemma empty_related_produces_derives {u v w : List (Symbol T g.NT)}
+lemma produces_nullableRelated_to_derives {u v w : List (Symbol T g.NT)}
     (huv : g.Produces u v) (hwv : NullableRelated w v) :
-    ∃ u', NullableRelated u' u ∧ g.eliminate_empty.Derives u' w := by
+    ∃ u', NullableRelated u' u ∧ g.eliminateEmpty.Derives u' w := by
   obtain ⟨r, hrg, hr⟩ := huv
   rw [r.rewrites_iff] at hr
   obtain ⟨p, q, hv, hw⟩ := hr
@@ -917,53 +885,53 @@ lemma empty_related_produces_derives {u v w : List (Symbol T g.NT)}
   | nil =>
     refine ⟨w, ?_, by rfl⟩
     rw [hv, hw]
-    apply (hw₁.append _).append hw₃
+    apply nullable_related_append (nullable_related_append hw₁ _) hw₃
     apply NullableRelated.empty_left
     apply Produces.trans_derives
-    apply rewrites_produces hrg
-    exact hw₂.empty_nullable
+    apply Produces.input_output hrg
+    exact hw₂.empty_nullableWord
   | cons d l =>
     use (w₁ ++ [Symbol.nonterminal r.input] ++ w₃)
     constructor
     · rw [hv]
-      exact (hw₁.append (by rfl)).append hw₃
+      exact nullable_related_append (nullable_related_append hw₁ (by rfl)) hw₃
     · rw [hw]
       have hdl : (d :: l) ≠ [] := by simp
-      have hrdl := nullableRelated_rule_in_rules hrg hw₂ hdl
+      have hrdl := nullableRelated_mem_eliminateEmpty_rules hw₂ hrg hdl
       exact Produces.single ⟨⟨r.input, d :: l⟩, hrdl, ContextFreeRule.rewrites_of_exists_parts _ w₁ w₃⟩
 
-lemma implies_eliminate_empty_related {u v : List (Symbol T g.NT)}
+lemma derivesIn_non_empty_to_nullableRelated_derives {u v : List (Symbol T g.NT)}
     (hv : v ≠ []) {m : ℕ} (huv : g.DerivesIn u v m) :
-    ∃ u', NullableRelated u' u ∧ g.eliminate_empty.Derives u' v := by
+    ∃ u', NullableRelated u' u ∧ g.eliminateEmpty.Derives u' v := by
   cases m with
   | zero =>
     cases huv
     use u
   | succ n =>
     obtain ⟨u, huv, hvw⟩ := huv.head_of_succ
-    obtain ⟨u', hru', huw'⟩ := @implies_eliminate_empty_related _ _ hv _ hvw
-    obtain ⟨v', hvrv', hpv'u'⟩ := empty_related_produces_derives huv hru'
+    obtain ⟨u', hru', huw'⟩ := derivesIn_non_empty_to_nullableRelated_derives hv hvw
+    obtain ⟨v', hvrv', hpv'u'⟩ := produces_nullableRelated_to_derives huv hru'
     exact ⟨v', hvrv', hpv'u'.trans huw'⟩
 
-lemma implies_eliminate_empty {w : List (Symbol T g.NT)} {n : g.NT} {hw : w ≠ []} {m : ℕ}
+lemma derivesIn_to_eliminateEmpty_derives {w : List (Symbol T g.NT)} {n : g.NT} {hw : w ≠ []} {m : ℕ}
     (hnwm : g.DerivesIn [Symbol.nonterminal n] w m) :
-    g.eliminate_empty.Derives [Symbol.nonterminal n] w := by
-  obtain ⟨w', hw, hww⟩ := implies_eliminate_empty_related hw hnwm
+    g.eliminateEmpty.Derives [Symbol.nonterminal n] w := by
+  obtain ⟨w', hw, hww⟩ := derivesIn_non_empty_to_nullableRelated_derives hw hnwm
   cases hw with
   | empty_left =>
     obtain ⟨_, _⟩ := hww.eq_or_head
     · contradiction
-    · apply Derives.empty_empty at hww
+    · apply Derives.of_empty at hww
       contradiction
   | cons_nterm_match hx _ =>
     cases hx
     exact hww
   | cons_nterm_nullable hxy hn =>
-  · rw [NullableRelated.empty_empty hxy] at hww
-    have := hww.empty_empty
+  · rw [NullableRelated.empty_right hxy] at hww
+    have := hww.of_empty
     contradiction
 
-theorem eliminate_empty_correct : g.language \ {[]} = g.eliminate_empty.language := by
+theorem eliminateEmpty_correct : g.language \ {[]} = g.eliminateEmpty.language := by
   unfold language Generates
   apply Set.eq_of_subset_of_subset
   · intro w hw
@@ -971,21 +939,21 @@ theorem eliminate_empty_correct : g.language \ {[]} = g.eliminate_empty.language
     obtain ⟨hw', hw''⟩ := hw
     rw [Set.mem_setOf_eq, g.derives_iff_derivesIn] at hw'
     obtain ⟨n, hgwn⟩ := hw'
-    apply implies_eliminate_empty
+    apply derivesIn_to_eliminateEmpty_derives
     · intro hw
       rw [List.map_eq_nil_iff] at hw
       rw [hw] at hw''
       contradiction
-    · simp only [eliminate_empty]
+    · simp only [eliminateEmpty]
       exact hgwn
   · intro w hw
     rw [Set.mem_setOf_eq] at hw
     rw [Set.mem_diff]
     constructor
-    · exact eliminate_empty_implies hw
+    · exact eliminateEmpty_derives_to_derives hw
     · rw [Set.not_mem_singleton_iff]
       intro hw'
-      apply derives_not_epsilon hw
+      apply eliminateEmpty_derives_not_empty hw
       exact List.cons_ne_nil _ []
       rw [hw', List.map_nil]
 
